theories/Ref/EnTreeSpecFacts.v
@@ -18,11 +18,828 @@ From EnTree Require Import
      Ref.Padded
      Ref.EnTreeSpecDefinition
      Ref.MRecSpec
+     Basics.QuantType
 .
 
 From Paco Require Import paco.
 
 Local Open Scope entree_scope.
+
+Ltac inj_existT := repeat match goal with
+                          | H:existT _ _ _ = _ |- _ => apply inj_pairT2 in H
+                          end.
+
+#[global] Hint Resolve monotone_refines_ : paco.
+
+#[global] Hint Constructors refinesF : entree_spec.
+Print Hint entree_spec.
+Section quant_elim1.
+Context (E1 E2 : Type) `{EncodingType E1} `{EncodingType E2}. 
+Context (RPre : Rel E1 E2) (RPost : PostRel E1 E2).
+Context (R1 R2 : Type) (RR : Rel R1 R2).
+Context (q : QuantEnc).
+Lemma refines_Vis_forallR : forall t k,
+             refines RPre RPost RR t (Vis (Spec_forall q) k) ->
+         forall a, refines RPre RPost RR t (k a).
+Proof.
+ intros t k Href a. punfold Href. red in Href. cbn in *. pstep. red.
+  remember (observe t) as ot. clear Heqot.
+  remember (VisF (Spec_forall q) k) as x.
+  hinduction Href before E1; intros; inv Heqx; inj_existT; subst; pclearbot; eauto with entree_spec.
+Qed.
+
+Lemma refines_existsL : forall t k,
+    refines RPre RPost RR (Vis (Spec_exists q) k) t ->
+    forall a, refines RPre RPost RR (k a) t.
+Proof.
+  intros t k Href a. punfold Href. red in Href. cbn in *. pstep. red.
+  remember (observe t) as ot. clear Heqot.
+  remember (VisF (Spec_exists q) k) as x.
+  hinduction Href before E1; intros; inv Heqx; inj_existT; subst; pclearbot; eauto with entree_spec.
+Qed.
+End quant_elim1.
+
+
+
+Section refinesF_inv.
+Context {E1 E2 : Type} `{EncodingType E1} `{EncodingType E2} {R1 R2 : Type} {q : QuantEnc}.
+Context (RPre : Rel E1 E2) (RPost : PostRel E1 E2) (RR : Rel R1 R2).
+
+(* A version of refinesF specialized to a forall on the left *)
+Inductive forallRefinesF (F : entree_spec E1 R1 -> entree_spec E2 R2 -> Prop)
+          (kphi1 : encodes q -> entree_spec E1 R1) : entree_spec' E2 R2 -> Prop := 
+  | forallRefines_forallR (qb : QuantEnc) kphi2 :
+    (forall b, forallRefinesF F kphi1 (observe (kphi2 b))) ->
+    forallRefinesF F kphi1 (VisF (Spec_forall qb) kphi2)
+  | forallRefines_forallL phi (a : encodes q) : 
+    refinesF RPre RPost RR F (observe (kphi1 a)) phi ->
+    forallRefinesF F kphi1 phi
+  | forallRefines_existsR qb kphi2 (b : encodes qb) : 
+    (forallRefinesF F kphi1 (observe (kphi2 b))) ->
+    forallRefinesF F kphi1 (VisF (Spec_exists qb) kphi2)
+  | forallRefines_TauR phi2 :
+    forallRefinesF F kphi1 (observe phi2) ->
+    forallRefinesF F kphi1 (TauF phi2)
+.
+(* A version of refinesF specialized to an exists on the left *)
+Inductive existsRefinesF (F : entree_spec E1 R1 -> entree_spec E2 R2 -> Prop)
+          (kphi2 : encodes q -> entree_spec E2 R2) : entree_spec' E1 R1 -> Prop := 
+  | existsRefines_existsR phi a :
+    refinesF RPre RPost RR F phi (observe (kphi2 a)) ->
+    existsRefinesF F kphi2 phi
+  | existsRefines_forallL (qb : QuantEnc) (kphi1 : encodes qb -> entree_spec E1 R1) (b : encodes qb):
+    existsRefinesF F kphi2 (observe (kphi1 b)) ->
+    existsRefinesF F kphi2 (VisF (@Spec_forall E1 qb) kphi1)
+  | existsRefines_existsL (qb : QuantEnc) (kphi1 : encodes qb -> entree_spec E1 R1) :
+    (forall b, existsRefinesF F kphi2 (observe (kphi1 b))) ->
+    existsRefinesF F kphi2 (VisF (@Spec_exists E1 qb) kphi1)
+  | existsRefines_TauL phi1 :
+    existsRefinesF F kphi2 (observe phi1) ->
+    existsRefinesF F kphi2 (TauF phi1)
+.
+
+Lemma refinesF_Vis_forallL : forall F (t : entree_spec' E2 R2) (k : encodes q -> entree_spec E1 R1),
+    refinesF RPre RPost RR F (VisF (@Spec_forall E1 q) k) t ->
+    forallRefinesF F k t.
+Proof.
+  intros. remember (VisF (Spec_forall q) k) as t1.
+  induction H1; try discriminate.
+  - constructor. auto.
+  - constructor. intros. auto.
+  - eapply forallRefines_existsR. eauto.
+  - inversion Heqt1. subst. inj_existT. subst.
+    econstructor. eauto.
+Qed.
+
+Lemma refinesF_Vis_existsR : forall F (t : entree_spec' E1 R1) (k : encodes q -> entree_spec E2 R2),
+    refinesF RPre RPost RR F t (VisF (@Spec_exists E2 q) k) ->
+    existsRefinesF F k t.
+Proof.
+  intros. remember (VisF (Spec_exists q) k) as t1.
+  induction H1; try discriminate.
+  - constructor. eauto.
+  - inversion Heqt1. subst. inj_existT. subst. econstructor. 
+    eauto.
+  - eapply existsRefines_forallL. eauto.
+  - constructor. eauto.
+Qed.
+
+End refinesF_inv.
+
+Section refines_tau_inv.
+Context (E1 E2 : Type) `{EncodingType E1} `{EncodingType E2}. 
+Context (RPre : Rel E1 E2) (RPost : PostRel E1 E2).
+Context (R1 R2 : Type) (RR : Rel R1 R2).
+
+Lemma refines_TauL_inv : forall phi1 phi2,
+    refines RPre RPost RR (Tau phi1) phi2 -> refines RPre RPost RR phi1 phi2.
+Proof.
+  pcofix CIH. intros. pstep. red. punfold H2. red in H2.
+  cbn in *. remember (TauF phi1) as x.
+  hinduction H2 before RPre; intros; inv Heqx; pclearbot; eauto with entree_spec.
+  constructor. pstep_reverse. eapply paco2_mon; try apply H1. intros. contradiction.
+  eapply monotone_refinesF. 2 : eauto. intros. pclearbot. left.
+  eapply paco2_mon; try apply PR. intros. contradiction.
+Qed.
+
+Lemma refines_TauR_inv : forall phi1 phi2,
+    refines RPre RPost RR phi1 (Tau phi2) -> refines RPre RPost RR phi1 phi2.
+Proof.
+  intros. pstep. red. punfold H1. red in H1.
+  cbn in *. remember (TauF phi2) as x.
+  hinduction H1 before RPre; intros; inv Heqx; pclearbot; eauto with entree_spec.
+  constructor. pstep_reverse.
+Qed.
+
+Lemma refinesF_TauR_inv : forall phi1 phi2,
+      refinesF RPre RPost RR (upaco2 (refines_ RPre RPost RR) bot2) (observe phi1) (TauF phi2) ->
+      refinesF RPre RPost RR (upaco2 (refines_ RPre RPost RR) bot2) (observe phi1) (observe phi2).
+Proof.
+  intros. pstep_reverse. apply refines_TauR_inv. pstep. auto.
+Qed.
+
+Lemma refinesF_TauL_inv : forall phi1 phi2,
+      refinesF RPre RPost RR (upaco2 (refines_ RPre RPost RR) bot2) (TauF phi1) (observe phi2) ->
+      refinesF RPre RPost RR (upaco2 (refines_ RPre RPost RR) bot2) (observe phi1) (observe phi2).
+Proof.
+  intros. pstep_reverse. apply refines_TauL_inv. pstep. auto.
+Qed.
+
+Lemma refinesF_Vis_existsR_Tau_inv : forall (q : QuantEnc) t (k : encodes q -> _),
+    existsRefinesF RPre RPost RR (upaco2 (refines_ RPre RPost RR) bot2) k (TauF t) ->
+    existsRefinesF RPre RPost RR (upaco2 (refines_ RPre RPost RR) bot2) k (observe t).
+Proof.
+  intros. inv H1; auto.
+  econstructor. eapply refinesF_TauL_inv. eauto.
+Qed.
+End refines_tau_inv.
+
+Create HintDb solve_padded.
+#[global] Hint Constructors refinesF : solve_padded.
+#[global] Hint Resolve padded_monotone_ : paco.
+Section paddedF_hints.
+Context (E : Type) `{EncodingType E}.
+
+
+Lemma paddedF_TauF_hint:
+  forall (R : Type) (phi1 : entree_spec E R), paddedF (upaco1 padded_ bot1) (TauF phi1) -> padded phi1.
+Proof.
+  intros R phi1. intros. inv H0. pclearbot. auto.
+Qed.
+
+Lemma paddedF_TauF_hint':
+  forall (R1 : Type) (phi1 : entree_spec E R1), paddedF (upaco1 padded_ bot1) (TauF phi1) -> paddedF (upaco1 padded_ bot1) (observe phi1).
+Proof.
+  intros. pstep_reverse. apply paddedF_TauF_hint. auto.
+Qed.
+
+Lemma paddedF_VisF_hint:
+  forall (R1 A : Type) (kphi : A -> entree E R1)
+     (e : E) ,
+    paddedF (upaco1 padded_ bot1) (VisF e kphi) -> forall a, padded (kphi a).
+Proof.
+  intros. pstep. red.
+  inv H0. inj_existT. subst. constructor. eauto.
+Qed.
+
+Lemma paddedF_VisF_hint':
+  forall (R1 A : Type) (kphi : A -> entree E R1)
+     (e : E) ,
+    paddedF (upaco1 padded_ bot1) (VisF e kphi) -> forall a, paddedF (upaco1 padded_ bot1) (observe (kphi a)).
+Proof.
+  pstep_reverse. apply paddedF_VisF_hint.
+Qed.
+
+Lemma padded_Tau_hint:
+  forall R3 e (k1 : encodes e -> entree_spec E R3) (b : encodes e), (forall a , paco1 padded_ bot1 (k1 a)) -> padded (Tau (k1 b)).
+Proof.
+  intros. pstep. constructor. left. auto.
+Qed.
+
+Lemma paddedF_Tau_inv_hint:
+  forall (R1 : Type) (phi1 : entree_spec E R1),
+    paddedF (upaco1 padded_ bot1) (observe phi1) -> paddedF (upaco1 padded_ bot1) (TauF phi1).
+Proof.
+  intros. constructor. left. pstep. auto.
+Qed.
+
+Lemma paddedF_Tau_Vis_hint:
+  forall  (R2: Type) (e : E) (a : encodes e) (kphi0 : encodes e -> entree E R2) (phi2 : entree E R2),
+    paddedF (upaco1 padded_ bot1) (TauF phi2) -> VisF e kphi0 = observe phi2 -> paddedF (upaco1 padded_ bot1) (TauF (kphi0 a)).
+Proof.
+  intros. inv H0. pclearbot. punfold H3. red in H3.
+  rewrite <- H1 in H3. inv H3. inj_existT. subst.
+  constructor. left. pstep. constructor. auto.
+Qed.
+
+Lemma paddedF_TauF_TauF_hint:
+  forall (R1 : Type) (phi phi1 : entree_spec E R1),
+    paddedF (upaco1 padded_ bot1) (TauF phi1) -> TauF phi = observe phi1 -> paddedF (upaco1 padded_ bot1) (TauF phi).
+Proof.
+  intros. inv H0. constructor. left. pclearbot. punfold H3. red in H3.
+  rewrite <- H1 in H3. inv H3. pclearbot. auto.
+Qed.
+
+Lemma paddedF_VisF_TauF_hint:
+  forall (E1 : Type) (Henc1 : EncodingType E1) (R1 : Type) (e : E1)
+    (k2 : encodes e -> entree E1 R1) (a : encodes e),
+    paddedF (upaco1 padded_ bot1) (VisF e k2) -> paddedF (upaco1 padded_ bot1) (TauF (k2 a)).
+Proof.
+  intros E1 Henc1 R1 A k2 a H1.
+  inversion H1. subst. inj_existT. subst. constructor.
+  left. pstep. constructor. auto.
+Qed.
+
+End paddedF_hints.
+
+Lemma rcompose_hint A B C (R1 : Rel A B) (R2 : Rel B C) a b c : 
+  R1 a b -> R2 b c -> rcompose R1 R2 a c.
+Proof.
+  intros. exists b. auto.
+Qed.
+
+#[local] Hint Resolve paddedF_TauF_hint : solve_padded.
+#[local] Hint Resolve paddedF_TauF_hint' : solve_padded.
+#[local] Hint Resolve paddedF_VisF_hint : solve_padded.
+#[local] Hint Resolve paddedF_VisF_hint' : solve_padded.
+(* hopefully this is *)
+#[local] Hint Resolve rcompose_hint : solve_padded.
+#[local] Hint Resolve padded_Tau_hint : solve_padded.
+#[local] Hint Unfold padded : solve_padded.
+#[local] Hint Unfold padded_ : solve_padded.
+#[local] Hint Resolve paddedF_Tau_inv_hint : solve_padded.
+#[local] Hint Resolve paddedF_Tau_Vis_hint : solve_padded.
+#[local] Hint Resolve  paddedF_TauF_TauF_hint : solve_padded.
+#[local] Hint Resolve paddedF_VisF_TauF_hint : solve_padded.
+
+Lemma refines_eutt_padded_l_tau_aux:
+  forall (E1 E2 : Type) `{EncodingType E1} `{EncodingType E2} (R2 : Type)
+    (R1 : Type) (RPre : Rel E1 E2)
+    (RPost : PostRel E1 E2) (RR : R1 -> R2 -> Prop)
+    (r : entree_spec E1 R1 -> entree_spec E2 R2 -> Prop)
+    (m1 m2 : entree_spec E1 R1) (t3 : entree_spec E2 R2),
+    (forall (t1 t2 : entree_spec E1 R1) (t4 : entree_spec E2 R2),
+        padded t2 ->
+        padded t4 -> t1 ≈ t2 -> refines RPre RPost RR t1 t4 -> r t2 t4) ->
+    paco2 (eqit_ eq true true id) bot2 m1 m2 ->
+    paddedF (upaco1 padded_ bot1) (TauF m2) ->
+    paddedF (upaco1 padded_ bot1) (observe t3) ->
+    refinesF RPre RPost RR (upaco2 (refines_ RPre RPost RR) bot2)
+             (TauF m1) (observe t3) ->
+    refinesF RPre RPost RR (upaco2 (refines_ RPre RPost RR) r)
+             (TauF m2) (observe t3).
+Proof.
+  intros E1 E2 Henc1 Henc2 R2 R1 RPre RPost RR r m1 m2 t3 CIH REL Hpad2 Hpad3 Href.
+  remember (observe t3) as ot3. clear Heqot3 t3.
+  assert (HDEC : (exists t4, ot3 = TauF t4) \/ (forall t4, ot3 <> TauF t4)).
+  { destruct ot3; eauto; right; repeat intro; discriminate. }
+  destruct HDEC as [ [t4 Ht4] |  Ht3]; subst.
+  {
+    constructor. right. eapply CIH; eauto. inv Hpad2. pclearbot. auto.
+    inv Hpad3. pclearbot. auto.
+    apply refines_TauL_inv. apply refines_TauR_inv. pstep. auto.
+  }
+  destruct ot3; try (exfalso; eapply Ht3; eauto; fail); try destruct e.
+  + inv Href. constructor. punfold REL. red in REL.
+    remember (RetF r0) as y. hinduction H0 before r; intros; inv Heqy; subst; eauto with entree_spec.
+    * remember (RetF r1) as x. hinduction REL before r; intros; inv Heqx; subst; eauto with entree_spec.
+    * eapply IHrefinesF; eauto. pstep_reverse. 
+      (* need to move tau_eutt and tau_euttge into this branch, *)
+      setoid_rewrite <- (tau_eutt t1). pstep. auto.
+    * inv Hpad2. pclearbot. punfold H1. red in H1.
+      remember (VisF (Spec_forall A) k) as x. hinduction REL before r; intros; inv Heqx; inj_existT; subst; 
+        eauto with solve_padded.
+      econstructor. eapply IHrefinesF; eauto. pclearbot. pstep_reverse. 
+      eauto with solve_padded.
+    * inv Hpad2. pclearbot. punfold H2. red in H2.
+      remember (VisF (Spec_exists A) k) as x. hinduction REL before r; intros; inv Heqx; inj_existT; subst; 
+        eauto with solve_padded.
+      econstructor. intros. pclearbot. eapply H0; eauto with solve_padded. pstep_reverse.
+
+      (* left off here *)
+  + inv Href. constructor.
+    inv Hpad2. pclearbot. punfold H1. red in H1. punfold REL. red in REL.
+    inv Hpad3. inj_existT. subst.
+    remember (VisF (Spec_vis e) (fun a : encodes (Spec_vis e)  => Tau (k1 a))) as y.
+    assert (Hy : paddedF (upaco1 padded_ bot1) y).
+    { subst. constructor. auto. }
+    hinduction H0 before r; intros; inv Heqy; inj_existT; subst; eauto with solve_padded.
+    (* * eapply IHrefinesF; eauto. pstep_reverse. rewrite <- (tau_eutt phi). pstep. auto. *)
+    * remember (VisF (Spec_vis e1) k1) as y. pclearbot.
+      (* shouldn't I know that k2 is padded here? *)
+      hinduction REL before r; intros; inv Heqy; inj_existT; subst.
+      -- pclearbot. constructor; auto. intros. eapply H0 in H3. destruct H3; try contradiction.
+         right. pclearbot. inv Hy. inj_existT. subst. eapply CIH; eauto with solve_padded; try apply REL. 
+         pstep. constructor. auto.
+      -- constructor. eapply IHREL; eauto.
+         inv H1. pclearbot. pstep_reverse.
+    * eapply IHrefinesF; eauto with solve_padded. pstep_reverse. rewrite <- (tau_eutt t1).
+      pstep. auto.
+    * remember (VisF (Spec_forall A) k) as x.
+      hinduction REL before r; intros; inv Heqx; inj_existT; subst; eauto with solve_padded.
+      econstructor. pclearbot. eapply IHrefinesF; eauto with solve_padded. pstep_reverse.
+    * remember (VisF (Spec_exists A) k) as x.
+      hinduction REL before r; intros; inv Heqx; inj_existT; subst; eauto with solve_padded.
+      econstructor. intros. eapply H0; eauto. pclearbot. pstep_reverse.
+      inv H1; inj_existT; subst. constructor. auto.
+  + inv Hpad3. inj_existT. subst. apply refinesF_forallR. intros. constructor.
+    right. eapply CIH; pclearbot; eauto with solve_padded.
+    inv Hpad2. pclearbot. eapply refines_TauR_inv. 
+    set (fun a => Tau (k2 a)) as k2'. assert (Tau (k2 a) = k2' a). auto.
+    rewrite H.
+    apply refines_Vis_forallR. unfold k2'. apply refines_TauL_inv. pstep. auto.
+  + inv Hpad3. inj_existT. subst.
+    assert ( refinesF RPre RPost RR
+                      (upaco2 (refines_ RPre RPost RR) bot2)
+                      (observe m1)
+                      (VisF (Spec_exists k0) (fun a => Tau (k2 a))) ).
+    { rewrite itree_eta'. pstep_reverse. apply refines_TauL_inv. pstep. auto. }
+    clear Href. rename H into Href. pclearbot.
+    eapply refinesF_Vis_existsR in Href. punfold REL. red in REL.
+    hinduction Href before r; intros; eauto.
+    * eapply refinesF_existsR. constructor. right.
+      eapply CIH; eauto with solve_padded. pstep. Unshelve. 3 : exact a. 3 : exact (go _ _ phi). 
+      red. auto. red. apply refines_TauR_inv. pstep. auto.
+    * inv Hpad2. pclearbot. punfold H1. red in H1.
+      remember (VisF (Spec_forall qb) kphi1) as x. remember (observe m2) as om2.
+      hinduction REL before r; intros; inv Heqx; inj_existT; subst.
+      -- inv H1. inj_existT. subst. constructor. rewrite <- Heqom2.
+         eapply refinesF_forallL. Unshelve. 2 : exact b. eapply IHHref; eauto.
+         pclearbot. pstep_reverse. rewrite <- (tau_eutt (k1 b)). auto.
+         constructor. auto.
+      -- constructor. rewrite <- Heqom2. inv H1. pclearbot. punfold H2.
+    * inv Hpad2. pclearbot. punfold H3. red in H3.
+      remember (VisF (Spec_exists qb) kphi1) as x. remember (observe m2) as om2.
+      hinduction REL before r; intros; inv Heqx; inj_existT; subst.
+      -- inv H3. inj_existT. subst. constructor. intros.
+         rewrite <- Heqom2. constructor. intros. eapply H0; eauto. Unshelve. all : auto.
+         pclearbot. pstep_reverse.  setoid_rewrite tau_eutt in REL. auto.
+         constructor. auto.
+      -- constructor. rewrite <- Heqom2.
+         eapply IHREL; eauto. inv H3. pclearbot. pstep_reverse.
+    * eapply IHHref; eauto. pstep_reverse. rewrite <- (tau_eutt phi1). pstep. auto.
+Qed.
+
+Lemma refines_eutt_padded_r_tau_aux:
+  forall (E1 E2 :Type) `{EncodingType E1} `{EncodingType E2} (R2 : Type)
+    (R1 : Type) (RPre : Rel E1 E2)
+    (RPost : PostRel E1 E2) (RR : R1 -> R2 -> Prop)
+    (r : entree_spec E1 R1 -> entree_spec E2 R2 -> Prop)
+    (m1 m2 : entree_spec E2 R2) (t1 : entree_spec E1 R1),
+    refinesF RPre RPost RR (upaco2 (refines_ RPre RPost RR) bot2)
+             (observe t1) (TauF m1) ->
+    paddedF (upaco1 padded_ bot1) (TauF m2) ->
+    paddedF (upaco1 padded_ bot1) (observe t1) ->
+    paco2 (eqit_ eq true true id) bot2 m1 m2 ->
+    (forall (t2 : entree_spec E1 R1) (t3 t4 : entree_spec E2 R2),
+        padded t2 ->
+        padded t4 -> t3 ≈ t4 -> refines RPre RPost RR t2 t3 -> r t2 t4) ->
+    refinesF RPre RPost RR (upaco2 (refines_ RPre RPost RR) r)
+             (observe t1) (TauF m2).
+Proof.
+  intros E1 E2 Henc1 Henc2 R2 R1 RPre RPost RR r m1 m2 t1 Href Hpad3 Hpad1 REL CIH.
+  remember (observe t1) as ot1. clear Heqot1 t1.
+  assert (HDEC : (exists t4, ot1 = TauF t4) \/ (forall t4, ot1 <> TauF t4)).
+  { destruct ot1; eauto; right; repeat intro; discriminate. }
+  destruct HDEC as [ [t4 Ht4] | Ht1]; subst.
+  { constructor. right. eapply CIH; eauto. inv Hpad1. pclearbot. auto.
+    inv Hpad3. pclearbot. auto. apply refines_TauL_inv.
+    apply refines_TauR_inv. pstep. auto. }
+  destruct ot1; try (exfalso; eapply Ht1; eauto; fail); try destruct e.
+  - inv Href. constructor. remember (RetF r0) as x.
+    punfold REL. red in REL. hinduction H1 before r; intros; inv Heqx; subst.
+    + remember (RetF r2) as x. hinduction REL before r; intros; inv Heqx; subst; eauto with solve_padded.
+    + eapply IHrefinesF; eauto. pstep_reverse. rewrite <- (tau_eutt t2).
+      pstep. auto.
+    + inv Hpad3. pclearbot. punfold H2. red in H2.
+      remember (VisF (Spec_forall A) k) as x.
+      hinduction REL before r; intros; inv Heqx; inj_existT; subst; pclearbot.
+      constructor. intros. eapply H0; eauto.  inv H2. inj_existT.
+      subst. constructor. left. pstep. constructor. auto.
+      pstep_reverse. constructor. eapply IHREL; eauto. inv H2. pclearbot. punfold H3.
+    + inv Hpad3. pclearbot. punfold H0. red in H0.
+      remember (VisF (Spec_exists A) k) as x.
+      hinduction REL before r; intros; inv Heqx; inj_existT; subst; pclearbot.
+      econstructor. Unshelve. all : auto. intros. eapply IHrefinesF; eauto.  inv H0. inj_existT.
+      subst. constructor. left. pstep. constructor. auto.
+      pstep_reverse. constructor. eapply IHREL; eauto. inv H0. pclearbot. pstep_reverse.
+  - inv Href. constructor. remember (VisF (Spec_vis e) k) as x.
+    inv Hpad3. pclearbot. punfold H0. red in H0. punfold REL. red in REL.
+    remember (VisF (Spec_vis e) k) as x.
+    hinduction H1 before r; intros; inv Heqx; inj_existT; subst; eauto with solve_padded.
+    + remember (VisF (Spec_vis e2) k2) as x.
+      hinduction REL before r; intros; inv Heqx; inj_existT; subst.
+      * constructor; auto. intros. eapply H0 in H2. right. pclearbot.
+        eapply CIH; eauto with solve_padded. 2 : apply REL. 2 : destruct H2; try contradiction; auto. 
+        inv Hpad1. inj_existT. subst. pstep.
+        constructor. auto.
+      * constructor. eapply IHREL; eauto. inv H1. pclearbot. pstep_reverse.
+    + eapply IHrefinesF; eauto. pstep_reverse. setoid_rewrite <- (tau_eutt t2).
+      pstep. auto.
+   + remember (VisF (Spec_forall A) k) as x.
+     hinduction REL before r; intros; inv Heqx; inj_existT; subst.
+     * constructor; intros. eapply H0; eauto. pclearbot. pstep_reverse.
+       inv H1. inj_existT. subst. constructor. auto.
+     * constructor. eapply IHREL; eauto. inv H1. pclearbot. pstep_reverse.
+   + remember (VisF (Spec_exists A) k) as x.
+     hinduction REL before r; intros; inv Heqx; inj_existT; subst; eauto with solve_padded.
+     econstructor; intros. Unshelve. all : auto. eapply IHrefinesF; eauto with solve_padded. 
+     pclearbot. pstep_reverse.
+  - inv Hpad1. inj_existT. subst.
+    assert (refines RPre RPost RR (Vis (Spec_forall k0) (fun a => Tau (k2 a))) m1).
+    { apply refines_TauR_inv. pstep. auto. }
+    clear Href. rename H into Href.
+    punfold Href. red in Href. inv Hpad3. pclearbot. punfold H1. red in H1.
+    apply refinesF_Vis_forallL in Href. punfold REL. red in REL.
+    hinduction Href before r; intros; pclearbot.
+    + constructor. remember (VisF (Spec_forall qb) kphi2) as x.
+      hinduction REL before r; intros; inv Heqx; inj_existT; subst.
+      * inv H2. inj_existT. subst. constructor. intros. eapply H0; auto.
+        Unshelve. all : auto. pclearbot. setoid_rewrite tau_eutt in REL. pstep_reverse.
+        pclearbot. pstep_reverse.
+      * constructor. eapply IHREL; eauto. inv H2. pclearbot. pstep_reverse.
+    + eapply refinesF_forallL. Unshelve. all : auto. constructor.
+      right. eapply CIH; eauto with solve_padded.
+      rewrite (itree_eta' phi) in REL. pstep. red. eauto.
+      apply refines_TauL_inv. pstep. auto.
+    + constructor. remember (VisF (Spec_exists qb) kphi2) as x.
+      hinduction REL before r; intros; inv Heqx; inj_existT; subst.
+      * inv H1. inj_existT. subst. eapply refinesF_existsR.
+        Unshelve. all : auto. cbn. eapply IHHref; eauto.
+        pclearbot. setoid_rewrite tau_eutt in REL.
+        pstep_reverse. pclearbot. pstep_reverse.
+      * constructor. eapply IHREL; eauto. inv H1. pclearbot.
+        pstep_reverse.
+    + eapply IHHref; eauto. pstep_reverse. setoid_rewrite <- (tau_eutt phi2).
+      pstep. auto.
+  - inv Hpad1. inj_existT. subst.
+    apply refinesF_existsL. intros. constructor. right. eapply CIH; eauto with solve_padded.
+    pclearbot. apply H0. inv Hpad3. pclearbot. auto.
+    set (fun a => Tau (k2 a)) as k2'. 
+    apply refines_TauL_inv.
+    assert (k2' a = Tau (k2 a)). auto. rewrite <- H.
+    eapply refines_existsL. unfold k2'. apply refines_TauR_inv. pstep. auto.
+Qed.
+
+
+Lemma refines_eutt_padded_l E1 E2 `{EncodingType E1} `{EncodingType E2} R1 R2 RPre RPost RR :
+  forall (t1 t2 : entree_spec E1 R1) (t3 : entree_spec E2 R2),
+    padded t2 -> padded t3 -> t1 ≈ t2 ->
+    refines RPre RPost RR t1 t3 -> refines RPre RPost RR t2 t3.
+Proof.
+  pcofix CIH. intros t1 t2 t3 Hpad2 Hpad3 Heutt Href.
+  punfold Hpad2. red in Hpad2.
+  punfold Hpad3. red in Hpad3.
+  punfold Heutt. red in Heutt.
+  punfold Href. red in Href. pstep.
+  red.
+  hinduction Heutt before r; intros; pclearbot; eauto.
+  - subst. rewrite itree_eta' at 1. pstep_reverse.
+    eapply paco2_mon; [ pstep; eapply Href | intros; contradiction].
+  - eapply refines_eutt_padded_l_tau_aux; eauto.
+  - (* need to figure this out *)
+    destruct e.
+    + assert (Hx : Vis (Spec_vis e) k1 ≈ Vis (Spec_vis e) k2).
+      pstep. constructor. left. auto.
+      punfold Hx. red in Hx. cbn in *.
+      remember (VisF (Spec_vis e) k1) as x.
+      hinduction Href before r; intros; inv Heqx; inj_existT; subst; eauto.
+      * constructor; auto. intros a b Hab.
+        eapply H2 in Hab. destruct Hab; try contradiction.
+        right. eapply CIH; eauto with solve_padded. inv Hpad2.
+        inj_existT. subst. pstep. constructor. auto.
+        inv Hpad3. inj_existT. subst. pstep. constructor. auto.
+        inv Hx. inj_existT. subst. destruct (REL0 a); try contradiction. auto.
+      * constructor. auto. eapply IHHref; eauto with solve_padded.
+      * constructor; auto. intros.
+        eapply H2; eauto with solve_padded.
+      * econstructor. eapply IHHref; eauto with solve_padded.
+    + inv Hpad2. inj_existT. subst. pclearbot.
+      eapply refinesF_Vis_forallL in Href.
+      induction Href.
+      * constructor. intros. eapply H3. eauto with solve_padded.
+      * econstructor. Unshelve. all : auto.
+        rewrite itree_eta'.
+        eapply refines_eutt_padded_l_tau_aux; eauto.
+        setoid_rewrite tau_eutt in REL. auto. constructor. left. auto.
+        constructor. auto.
+      * eapply refinesF_existsR. eapply IHHref; eauto with solve_padded. inv Hpad3.
+        inj_existT. subst. constructor. auto.
+      * constructor. eapply IHHref. inv Hpad3. pclearbot. pstep_reverse.
+    + inv Hpad2. inj_existT. subst.
+      (* this should be fine, exists L is invertible and then I just
+         further invert Href until I learn more about t3
+       *)
+      constructor. intros.
+      assert (forall a, refinesF RPre RPost RR (upaco2 (refines_ RPre RPost RR) bot2) (observe (k1 a)) (observe t3)).
+      intros. pstep_reverse. eapply refines_existsL. pstep. auto.
+      clear Href. rename H1 into Href. specialize (Href a).
+      eapply refines_eutt_padded_l_tau_aux; eauto.
+      setoid_rewrite tau_eutt in REL. auto.
+      constructor. auto. constructor. auto.
+  - eapply IHHeutt; eauto.
+    pstep_reverse. apply refines_TauL_inv. pstep. auto.
+  - constructor. eapply IHHeutt; eauto with solve_padded.
+Qed.
+
+
+
+Lemma refines_eutt_padded_r E1 E2 `{EncodingType E1} `{EncodingType E2} R1 R2 RPre RPost RR :
+  forall (t1 : entree_spec E1 R1) (t2 t3 : entree_spec E2 R2),
+    padded t1 -> padded t3 -> t2 ≈ t3 ->
+    refines RPre RPost RR t1 t2 -> refines RPre RPost RR t1 t3.
+Proof.
+  pcofix CIH. intros t1 t2 t3 Hpad1 Hpad3 Heutt Href.
+  punfold Href. punfold Heutt. red in Heutt. red in Href.
+  punfold Hpad1. red in Hpad1. punfold Hpad3. red in Hpad3.
+  pstep. red. hinduction Heutt before r; intros; pclearbot.
+  - subst. rewrite itree_eta'. pstep_reverse.
+    eapply paco2_mon; [ pstep; eapply Href | intros; contradiction].
+  - eapply refines_eutt_padded_r_tau_aux; eauto.
+  - destruct e.
+    + assert (Hx : Vis (Spec_vis e) k1 ≈ Vis (Spec_vis e) k2).
+      pstep. constructor. left. auto. punfold Hx. red in Hx.
+      cbn in Hx.
+      remember (VisF (Spec_vis e) k1) as y.
+      hinduction Href before r; intros; inv Heqy; inj_existT; subst; eauto with solve_padded.
+      constructor. auto. right. eapply CIH; eauto with solve_padded.
+      inv Hpad1. inj_existT. subst. pstep. constructor. auto.
+      inversion Hx. subst. inj_existT. subst. destruct (REL0 b); try contradiction; try apply H4.
+      apply H2 in H3. destruct H3; auto; try contradiction.
+    + inv Hpad3. inj_existT. subst.
+      constructor. intros.
+      eapply refines_eutt_padded_r_tau_aux with (m1 := k1 a); auto.
+      constructor. pstep_reverse. apply refines_Vis_forallR. pstep. auto.
+      constructor. auto. setoid_rewrite tau_eutt in REL. auto.
+    + eapply refinesF_Vis_existsR in Href.
+      hinduction Href before r; intros; eauto.
+      * econstructor. inv Hpad3. inj_existT. subst.
+        Unshelve. all : auto. cbn.
+        rewrite itree_eta' at 1.
+        eapply refines_eutt_padded_r_tau_aux; auto. eauto.
+        constructor. eauto.
+        constructor. auto. setoid_rewrite tau_eutt in REL. auto.
+      * eapply refinesF_forallL. eapply IHHref; eauto.
+        inv Hpad1. inj_existT. subst. constructor. auto.
+      * apply refinesF_existsL. intros. eapply H2; eauto.
+        inv Hpad1. inj_existT. subst. constructor. auto.
+      * constructor. eapply IHHref; eauto. inv Hpad1. pclearbot. pstep_reverse.
+  - eapply IHHeutt; eauto. pstep_reverse. apply refines_TauR_inv. pstep. auto.
+  - constructor. eapply IHHeutt; eauto. inv Hpad3. pclearbot. pstep_reverse.
+Qed.
+
+Lemma Spec_vis_inv:
+  forall (E1 R1 : Type) (H : EncodingType E1) (E2 R2 : Type) (H0 : EncodingType E2)
+    (RPre1 : Rel E1 E2) (RPost1 : PostRel E1 E2) (RR1 : Rel R1 R2) (e3 : E2)
+    (k1 : encodes (Spec_vis e3) -> entree_spec E2 R2) (e0 : E1) (k0 : encodes (Spec_vis e0) -> entree_spec E1 R1),
+    padded ((Vis (Spec_vis e0) k0)) -> padded (Vis (Spec_vis e3) k1 : entree_spec E2 R2) ->
+    refinesF RPre1 RPost1 RR1 (upaco2 (refines_ RPre1 RPost1 RR1) bot2) (VisF (Spec_vis e0) k0)
+             (VisF (Spec_vis e3) k1) ->
+    forall (a : encodes e0) (c : encodes e3),
+      RPost1 e0 e3 a c -> refines RPre1 RPost1 RR1 (k0 a) (k1 c).
+Proof.
+  intros E1 R1 H E2 R2 H0 RPre1 RPost1 RR1 e3 k1 e0 k0 Hpad1 Hpad2 Href a c H6.
+  remember (VisF (Spec_vis e0) k0) as x.
+  remember (VisF (Spec_vis e3) k1) as y. cbn in *.
+  hinduction Href before E1; intros; try discriminate.
+  inversion Heqx. subst.
+  assert (padded (Vis (Spec_vis e0) k3)).
+  setoid_rewrite <- Heqx. auto.
+  assert (padded (Vis (Spec_vis e3) k0)).
+  setoid_rewrite <- Heqy. auto.
+  assert (forall a : encodes (Spec_vis e0), k1 a ≅ k3 a).
+  {
+    eapply eqit_Vis_inv. setoid_rewrite Heqx. reflexivity.
+  }
+  inversion Heqy. subst.
+  assert (forall a : encodes (Spec_vis e3), k2 a ≅ k0 a).
+  {
+    eapply eqit_Vis_inv. setoid_rewrite Heqy. reflexivity.
+  }
+  eapply refines_eutt_padded_l; eauto.
+  eapply H2 in H6. pclearbot. 
+  pinversion H3. subst. inj_existT. subst. pstep. constructor. auto.
+  pinversion H4. subst. inj_existT. subst. pstep. constructor. auto.
+  rewrite <- H5. reflexivity.
+  eapply refines_eutt_padded_r; eauto.
+  pinversion Hpad1. subst. inj_existT. subst. pstep. constructor.
+  auto.
+  pinversion H4. subst. inj_existT. subst. pstep. constructor.
+  auto. rewrite <- H7. reflexivity.
+  apply H2 in H6. pclearbot. auto.
+Qed.
+
+Lemma refinesTrans_aux:
+  forall (E3 R3 : Type) (H1 : EncodingType E3) (E1 R1 : Type) (H : EncodingType E1) (E2 R2 : Type)
+    (H0 : EncodingType E2) (RPre1 : Rel E1 E2) (RPre2 : Rel E2 E3) (RPost1 : PostRel E1 E2)
+    (RPost2 : PostRel E2 E3) (RR1 : Rel R1 R2) (RR2 : Rel R2 R3)
+    (r : Rel (entree_spec E1 R1) (entree_spec E3 R3)) (t1 : entree_spec E1 R1) (t0 : entree_spec E2 R2)
+    (e : SpecEvent E3) (k1 : encodes e -> entree (SpecEvent E3) R3),
+    (forall (t2 : entree_spec E1 R1) (t3 : entree_spec E2 R2) (t4 : entree_spec E3 R3),
+        padded t2 ->
+        padded t3 -> padded t4 -> refines RPre1 RPost1 RR1 t2 t3 -> refines RPre2 RPost2 RR2 t3 t4 -> r t2 t4) ->
+    paco2 (refines_ RPre1 RPost1 RR1) bot2 t1 t0 ->
+    paddedF (upaco1 padded_ bot1) (TauF t1) ->
+    paddedF (upaco1 padded_ bot1) (TauF t0) ->
+    refinesF RPre2 RPost2 RR2 (upaco2 (refines_ RPre2 RPost2 RR2) bot2) (TauF t0)
+             (VisF e (fun a : encodes e => Tau (k1 a))) ->
+    (forall a : encodes e, upaco1 padded_ bot1 (k1 a)) ->
+    refinesF (rcompose RPre1 RPre2) (RComposePostRel RPre1 RPre2 RPost1 RPost2) (rcompose RR1 RR2)
+             (upaco2 (refines_ (rcompose RPre1 RPre2) (RComposePostRel RPre1 RPre2 RPost1 RPost2) (rcompose RR1 RR2)) r)
+             (TauF t1) (VisF e (fun a : encodes e => Tau (k1 a))).
+Proof.
+  intros E3 R3 H1 E1 R1 H E2 R2 H0 RPre1 RPre2 RPost1 RPost2 RR1 RR2 r t1 t0 e k1.
+  intros CIH Ht10 Ht1 Ht0 Ht23 Hk1.
+  destruct e.
+  - inv Ht23. rename H3 into Ht23. constructor.
+    punfold Ht10. red in Ht10.
+    assert (Hy : padded (Vis (Spec_vis e) (fun a : encodes (Spec_vis e) => Tau (k1 a)))).
+    pstep. constructor. auto. punfold Hy. red in Hy. cbn in *.
+    remember ((fun a => Tau (k1 a))) as k1'. assert (forall a, padded (k1' a)).
+    pclearbot. auto. pstep. red. cbn. subst. constructor. auto.
+    clear Heqk1' Hk1 k1. rename k1' into k1.
+    inv Ht1. inv Ht0. pclearbot. punfold H4. punfold H5. red in H4. red in H5.
+    remember (VisF (Spec_vis e) k1) as y. (* at this point need to prove that go _ _ y is padded*)
+    hinduction Ht23 before r; intros; inv Heqy; inj_existT; subst; eauto with solve_padded.
+    + assert (refines RPre2 RPost2 RR2 (Vis (Spec_vis e1) k1) (Vis (Spec_vis e) k2)).
+      pstep. constructor. auto. auto.
+      clear H3. punfold H7. red in H7. cbn in H7.
+      remember (VisF (Spec_vis e1) k1) as x. cbn in *.
+      hinduction Ht10 before r; intros; inv Heqx; inj_existT; subst; eauto with solve_padded.
+      constructor; eauto with solve_padded. intros.
+      inv H9. inj_existT. subst.
+      specialize (H14 e0 H2 H4) as [c [Hc1 Hc2]].
+      right. eapply CIH; eauto with solve_padded.
+      all : try (inv H6; inv Hy; inj_existT; subst; pstep; constructor; auto; fail).
+      eapply H3 in Hc1; eauto. destruct Hc1; eauto. contradiction.
+      eapply Spec_vis_inv. pstep. auto. pstep. auto. eauto. eauto.
+    + eapply IHHt23; eauto with solve_padded. apply refinesF_TauR_inv. auto.
+    + eapply IHHt23; eauto with solve_padded. pstep_reverse. eapply refines_Vis_forallR. pstep. auto.
+    + eapply refinesF_Vis_existsR in Ht10. assert (Hk : forall a, padded (k a)). inv H6. inj_existT.
+      subst. intros. pstep. constructor. auto.
+      induction Ht10.
+      * rewrite itree_eta' at 1. eapply H3; eauto with solve_padded.
+      * econstructor. eapply IHHt10; eauto. inv H5. inj_existT. subst. constructor. auto.
+      * constructor. intros. eapply H8; eauto with solve_padded.
+      * constructor. eauto with solve_padded.
+  - apply refinesF_forallR. intros. constructor. right. eapply CIH; eauto with solve_padded.
+    pclearbot. apply Hk1. apply refines_TauL_inv. apply refines_TauR_inv.
+    set (fun a => Tau (k1 a)) as k'. assert (Tau (k1 a) = k' a). auto. rewrite H2.
+    apply refines_Vis_forallR. pstep. auto.
+  - rewrite itree_eta' in Ht23. apply refinesF_TauL_inv in Ht23. cbn in Ht23.
+    punfold Ht10. red in Ht10. inv Ht1. inv Ht0. pclearbot.
+    punfold H3. punfold H4. red in H3. red in H4. eapply refinesF_Vis_existsR in Ht23.
+    remember (observe t1) as ot1. remember (observe t0) as ot0.
+    remember (fun a => Tau (k1 a)) as k'.
+    hinduction Ht23 before r; intros; subst.
+    + eapply refinesF_existsR. Unshelve. all : auto. constructor.
+      right. eapply CIH; eauto with solve_padded. pstep. auto.
+      apply refines_TauR_inv. pstep. auto.
+    + inv H4. inj_existT. subst. pclearbot. cbn in Ht23.
+      assert (Hk2 : forall a, refinesF RPre1 RPost1 RR1  (upaco2 (refines_ RPre1 RPost1 RR1) bot2) (observe t1) (observe (k2 a)) ).
+      { cbn. intros. eapply refinesF_TauR_inv. set (fun a => Tau (k2 a)) as k2'.
+        assert (TauF (k2 a) = observe (k2' a)). auto. rewrite H2. 
+        pstep_reverse. eapply refines_Vis_forallR. pstep. auto. }
+      apply refinesF_Vis_existsR_Tau_inv in Ht23.
+      specialize (Hk2 b). specialize (H5 b). punfold H5. red in H5.
+      eapply IHHt23; eauto with solve_padded.
+    + inv H5. inj_existT. subst. pclearbot.
+      apply refinesF_Vis_existsR in Ht10.
+      assert (Hk2 : forall b, existsRefinesF RPre2 RPost2 RR2 (upaco2 (refines_ RPre2 RPost2 RR2) bot2)
+         (fun a : encodes k => Tau (k1 a)) (observe ((k2 b)))).
+      {
+        intros. apply refinesF_Vis_existsR_Tau_inv. apply H2.
+      }
+      clear H2.
+      remember (observe t1) as ot1. pclearbot.
+      remember (fun a => Tau (k2 a)) as k'.
+      assert (go _ _ ot1 ≈ t1). subst. rewrite <- itree_eta. reflexivity.
+      assert (Ht1 : padded t1). pstep. red. rewrite <- Heqot1. auto.
+      clear Heqot1.
+      hinduction Ht10 before r; intros; subst.
+      * eapply H3; eauto with solve_padded. Unshelve. all : auto.
+        pstep_reverse. eapply refines_eutt_padded_l; eauto with solve_padded.
+        pstep. constructor. auto.
+        pstep. auto. pstep_reverse. constructor. auto.
+      * inv H4. inj_existT. subst. pclearbot. constructor.
+        punfold H2. red in H2. cbn in *.
+        punfold Ht1. red in Ht1.
+        remember (VisF (Spec_forall qb0) (fun a => Tau (k3 a)) : entree_spec' E1 R1) as x.
+        cbn in Heqx. setoid_rewrite <- Heqx in H2.
+        remember (observe t1) as ot1. clear Heqot1 t1. pclearbot.
+        remember (fun a => Tau (k3 a)) as k3'.
+        hinduction H2 before r; intros; try (exfalso; inv Heqx; fail).
+        -- pclearbot. subst. inv Heqx. inj_existT. subst.
+           inv Ht1. inj_existT. subst.
+           eapply refinesF_forallL. Unshelve. all : auto.
+           eapply IHHt10; eauto with solve_padded.
+           constructor. auto. clear - REL.
+           specialize (REL b). setoid_rewrite REL. rewrite tau_eutt. reflexivity.
+           pclearbot. apply H4.
+        -- constructor. eapply IHeqitF; eauto with solve_padded.
+      * inv H5. inj_existT. subst. constructor. punfold H6. red in H6.
+        cbn in H6. punfold Ht1. red in Ht1.
+        remember (VisF (Spec_exists qb0) (fun a => Tau (k3 a)) : entree_spec' E1 R1) as x.
+        cbn in Heqx. setoid_rewrite <- Heqx in H6.
+        remember (fun a : encodes qb0 => Tau (k3 a)) as k3'.
+        hinduction H6 before r; intros; inv Heqx; inj_existT; subst.
+        -- inv Ht1. inj_existT. subst. constructor. cbn. intros.
+           eapply H3; eauto with solve_padded. Unshelve. all : auto.
+           constructor. auto. cbn. pclearbot. setoid_rewrite REL. apply tau_eutt.
+           pclearbot. apply H6.
+        -- constructor. eapply IHeqitF; eauto with solve_padded. auto.
+      * eapply IHHt10; eauto with solve_padded. rewrite <- itree_eta. rewrite <- H2.
+        rewrite tau_eutt. reflexivity.
+    + eapply IHHt23; eauto with solve_padded. apply refinesF_TauR_inv. auto.
+Qed.
+
+Theorem refinesTrans {E1 E2 E3 R1 R2 R3} `{EncodingType E1} `{EncodingType E2} `{EncodingType E3} RPre1 RPre2 RPost1 RPost2
+        (RR1 : R1 -> R2 -> Prop) (RR2 : R2 -> R3 -> Prop)
+        (t1 : entree_spec E1 R1) (t2 : entree_spec E2 R2) (t3 : entree_spec E3 R3):
+  padded t1 -> padded t2 -> padded t3 ->
+  refines RPre1 RPost1 RR1 t1 t2 -> refines RPre2 RPost2 RR2 t2 t3 ->
+  refines (rcompose RPre1 RPre2) (RComposePostRel RPre1 RPre2 RPost1 RPost2)
+          (rcompose RR1 RR2) t1 t3.
+Proof.
+  revert t1 t2 t3; pcofix CIH.
+  intros t1 t2 t3  Ht1 Ht2 Ht3 Ht12 Ht23.
+  pfold. red. punfold Ht12. red in Ht12.
+  punfold Ht23. red in Ht23. punfold Ht3. red in Ht3.
+  punfold Ht2. red in Ht2.
+  punfold Ht1. red in Ht1.
+  remember (observe t3) as ot3.  clear t3 Heqot3.
+  remember (observe t1) as ot1. clear t1 Heqot1.
+  hinduction Ht12 before r; intros.
+  - remember (RetF r2) as x. clear Ht2 Ht3.
+    hinduction Ht23 before r; intros; inv Heqx; eauto with solve_padded.
+  - pclearbot.
+    assert (Hdec : (exists t4, ot3 = TauF t4) \/ (forall t4, ot3 <> TauF t4)).
+    { destruct ot3; eauto; right; repeat intro; discriminate. }
+    destruct Hdec as [ [t4 Ht4] | Ht4 ]; subst.
+    + constructor. right. eapply CIH; eauto with solve_padded.
+      apply refines_TauL_inv. apply refines_TauR_inv. pstep. auto.
+    + destruct ot3; try (exfalso; eapply Ht4; eauto; fail).
+      * constructor. inv Ht23. clear Ht2 Ht3.
+        inv Ht1. pclearbot. punfold H2.
+        red in H2.
+        punfold H5. red in H5. remember (RetF r0) as y.
+        remember (observe t0) as ot0.
+        hinduction H4 before r; intros; inv Heqy; eauto with solve_padded.
+        -- remember (RetF r1) as y.
+           remember (observe t1) as ot1. clear Heqot1.
+           hinduction H3 before r; intros; inv Heqy; eauto with solve_padded.
+        -- eapply IHrefinesF; eauto.
+           pstep_reverse. apply refines_TauR_inv. pstep. auto.
+        -- eapply IHrefinesF; eauto. pstep_reverse.
+           eapply refines_Vis_forallR. pstep. auto.
+        -- eapply refinesF_Vis_existsR in H4.
+           induction H4; eauto with solve_padded.
+           rewrite itree_eta' at 1. eapply H3; eauto with solve_padded.
+           econstructor. eapply IHexistsRefinesF. inv H5. inj_existT.
+           subst. constructor. auto.
+      * inv Ht3. inj_existT. subst. eapply refinesTrans_aux; eauto.
+  - assert (Href : refines RPre1 RPost1 RR1 (Vis (Spec_vis e1) k1) (Vis (Spec_vis e2) k2)).
+    pstep. red. constructor. auto. auto. punfold Href. red in Href. cbn in *.
+    remember (VisF (Spec_vis e2) k2) as x.
+    (*k2 is getting captured in a weird way here from H3, 
+      need to ter
+     *)
+
+    hinduction Ht23 before r; intros; inv Heqx; inj_existT; subst; eauto.
+    + (*k1 and k3 are the same thing here *)
+      constructor. eauto with solve_padded. intros.
+      inv H6. inj_existT. subst.
+      specialize (H11 e3 H4 H2) as [c [? ?]].
+      right. eapply CIH. (* k3 vs k1?, might be an artifact of my recursion *) eauto with solve_padded. inv Ht1. inj_existT. subst. pstep. constructor. auto.
+      Unshelve. all : try apply (k1 c). inversion Ht2.
+      inj_existT. subst. pstep. constructor. auto.
+      inv Ht3. inj_existT. subst. pstep. constructor. auto.
+      apply Spec_vis_inv. pstep. auto. pstep. auto. auto. auto. apply H3 in H7. destruct H7; auto. contradiction.
+    + constructor. eapply IHHt23; eauto with solve_padded.
+    + pclearbot. constructor. intros. eapply H3; eauto with solve_padded.
+    + econstructor. eapply IHHt23; eauto with solve_padded.
+  - constructor. eapply IHHt12; eauto with solve_padded.
+  - eapply IHHt12; eauto with solve_padded. 
+    rewrite itree_eta'.
+    apply refinesF_TauL_inv. auto.
+  - apply refinesF_Vis_forallL in Ht23.
+    induction Ht23.
+    + constructor. intros. eauto with solve_padded.
+    + eapply H3; eauto with solve_padded.
+    + econstructor. eapply IHHt23; eauto with solve_padded.
+      inv Ht3. inj_existT. subst. constructor. auto.
+    + constructor. eapply IHHt23; eauto with solve_padded.
+  - eapply IHHt12; eauto with solve_padded. rewrite itree_eta'.
+    pstep_reverse. apply refines_existsL.
+    pstep. auto.
+  - econstructor. eapply IHHt12; eauto with solve_padded.
+  - constructor. intros. eapply H3; eauto with solve_padded.
+Qed.
+
+ 
+ 
+
+
 
 Definition padded_refines {E1 E2} `{EncodedType E1} `{EncodedType E2}
            {R1 R2 : Type} (RPre : Rel E1 E2) (RPost : PostRel E1 E2) (RR : Rel R1 R2)
